
$\displaystyle \frac{dS_c}{dt} = - \beta_c \ S_c \ (\alpha_c \ I)$ ...... (4)<br>
<br>
$\displaystyle \frac{dI_c}{dt} = \beta_c \ S_c \ (\alpha_c \ I) - \gamma \ I_c$ ...... (5)<br>
<br>
$\displaystyle \frac{dR_c}{dt} = \gamma \ I_c$ ...... (6)<br>
<br>
$\displaystyle \frac{dS_a}{dt} = - \beta_a \ S_a \ (\alpha_a \ I)$ ...... (7)<br>
<br>
$\displaystyle \frac{dI_a}{dt} = \beta_a \ S_a \ (\alpha_a \ I) - \gamma \ I_a$ ...... (8)<br>
<br>
$\displaystyle \frac{dR_a}{dt} = \gamma \ I_a$ ...... (9)<br>
<br>
$\displaystyle \frac{dS_e}{dt} = - \beta_e \ S_e \ (\alpha_e \ I)$ ...... (10)<br>
<br>
$\displaystyle \frac{dI_e}{dt} = \beta_e \ S_e \ (\alpha_e \ I) - \gamma \ I_e$ ...... (11)<br>
<br>
$\displaystyle \frac{dR_e}{dt} = \gamma \ I_e$ ...... (12)<br>
<br>
$(I = I_c + I_a + I_e)$<br>
<br>
$([\beta_c\ ,\ \beta_a\ ,\ \beta_e] = (\beta / N) [N_c\ ,\ N_a\ ,\ N_e])$<br>

